\begin{definition}
  Let $(M, \omega)$ be a symplectic manifold, $H \in \mathcal{F} M$.
  We say that $(M, \omega, H)$ is a \textbf{Hamiltonian system}. 
\end{definition}
\begin{definition}
  Let
    $M$ be a manifold,
    $H \in \mathcal{F} M$,
    $G$ be a Lie group,
    $\rho \colon G \to \Aut M$ be a group action.
  We say that $\rho$ \textbf{leaves $H$ invariant} if for any $g \in G$,
  \begin{equation}
    H \circ \rho_g = H.
  \end{equation}
\end{definition}
\begin{definition}
  Let
    $(M, \omega, H)$ be a Hamiltonian system,
    $G$ be a Lie group with Lie algebra $\mathfrak{g}$,
    $\rho \colon G \to \Aut M$ be a group action leaving $H$ invariant.
  Define $\gamma \colon \mathfrak{g} \to \mathfrak{X} M$ as follows:
  for $A \in \mathfrak{g}$, $x \in M$,
  \begin{equation}
    \gamma^A x
    := - \restrict{\frac{d}{d t}}{t = 0}(t \mapsto \rho_{(\exp(t A)} x).
  \end{equation}
  Let $\hat{J} \colon \mathfrak{g} \to \mathcal{F} M$ satisfies
  \begin{equation}
    \hamiltonian_H \circ \hat{J} = \gamma.
  \end{equation}
  Define the \textbf{momentum map} $J \colon M \to \mathfrak{g}^*$ as follows:
  for any $x \in M$, $A \in \mathfrak{g}$,
  \begin{equation}
    (J x) A = \hat{J}^A x.
  \end{equation}
\end{definition}
\begin{theorem}[Noether]
  Let
    $(M, \omega, H)$ be a Hamiltonian system,
    $G$ be a Lie group with Lie algebra $\mathfrak{g}$,
    $\rho \colon G \to \Aut(M)$ be a group action that leaves $H$ invariant,
    $\gamma \colon \mathfrak{g} \to \mathfrak{X} M$ and
    $\hat{J} \colon \mathfrak{g} \to \mathcal{F} M$ be constructed as above,
    $J \colon M \to \mathfrak{g}^*$ be the corresponding momentum map,
    $\varphi \colon \R \to \Aut M$ be the flow of $\hamiltonian_H$.
  Then $J$ leaves the flow of $\hamiltonian_H$ invariant.
  In other words, for any $t \in \R$,
  \begin{equation}
    J \circ \varphi_t = J.
  \end{equation}
\end{theorem}
\begin{proof}
  Let $A \in \mathfrak{g}$, $x \in M$ 
  \begin{equation}
    \poisson{\hat{J}^A}{H}(x)
    = {\restrict{\hamiltonian_{\hat{J}(A)}} H}(x)
    = (\gamma^A H)(x)
    = \restrict{\frac{d}{d t}}{t = 0} H(\rho_{\exp(t A)} x)
    = \restrict{\frac{d}{d t}}{t = 0} H(x)
    = 0.
  \end{equation}
  Hence, $\hat{J}^A \circ \varphi_t$ is constant.
  Therefore,
  \begin{equation}
    \hat{J}^A \circ \varphi_t = \hat{J}^A \circ \varphi_0 = \hat{J}^A.
  \end{equation}
  As a result,
  \begin{equation}
    (J(\varphi_t(x))) A
    = \hat{J}^A(\varphi_t(x))
    = \hat{J}^A(x)
    = (J x) A.
  \end{equation}
  Since $A$ and $x$ are arbitrary, $J \circ \varphi_t = J$, as wanted.
\end{proof}
