\begin{example}
  The following are computations of the exterior derivative in flat space.
  \begin{enumerate}
    \item
      \textbf{Exterior derivative in $\R^2$.}
      Let $x^1, x^2 \colon \R^2 \to \R$ be the coordinate maps.
      \begin{enumerate}
        \item
          \textbf{Exterior derivative of $0$-forms.}
          Consider a $0$-form (a function)
          $f \in \Omega^1(\R^2) = \mathcal{F}(\R^2)$.
          Then
          \begin{equation}
            d_0 f
            = \frac{\partial f}{\partial x^1}\, d x^1
            + \frac{\partial f}{\partial x^2}\, d x^2.
          \end{equation}
        \item
          \textbf{Exterior derivative of $1$-forms.}
          Consider a $1$-form $\omega \in \Omega^1(\R^2)$ such that
          $\omega = f_1\, d x^1 + f_2\, d x^2$,
          for some $f_1, f_2 \in \mathcal{F}(\R^2)$.
          Then
          \begin{equation}
            \begin{split}
              d_1 \omega
              & = d f_1 \wedge d x^1 + d f_2 \wedge d x^2 \\
              & =
                \left(
                  \frac{\partial f_1}{\partial x^1}\, d x^1
                  + \frac{\partial f_1}{\partial x^2}\, d x^2
                \right)
                \wedge d x^1
                +
                \left(
                  \frac{\partial f_2}{\partial x^1}\, d x^1
                  + \frac{\partial f_2}{\partial x^2}\, d x^2
                \right)
                \wedge d x^2 \\
              & =
                \left(
                  \frac{\partial f_2}{\partial x^1}
                  - \frac{\partial f_1}{\partial x^2}
                \right)\,
                d x^1 \wedge d x^2.
            \end{split}
          \end{equation}
      \end{enumerate}
    \item
      \textbf{Exterior derivative in $\R^3$.}
      Let $x^1, x^2, x^3 \colon \R^3 \to \R$ be the coordinate maps.
      \begin{enumerate}
        \item
          \textbf{Exterior derivative of $0$-forms.}
          Consider a $0$-form (a function)
          $f \in \Omega^1(\R^3) = \mathcal{F}(\R^3)$.
          Then
          \begin{equation}
            d_0 f
            = \frac{\partial f}{\partial x^1}\, d x^1
            + \frac{\partial f}{\partial x^2}\, d x^2
            + \frac{\partial f}{\partial x^3}\, d x^3.
          \end{equation}
        \item
          \textbf{Exterior derivative of $1$-forms.}
          Consider a $1$-form $\omega \in \Omega^1(\R^3)$ such that
          $\omega = f_1\, d x^1 + f_2\, d x^2 + f_3\, d x^3$,
          for some $f_1, f_2, f_3 \in \mathcal{F}(\R^3)$.
          Then
          \begin{equation}
            \begin{split}
              d_1 \omega
              & = d f_1 \wedge d x^1 + d f_2 \wedge d x^2 + d f_3 \wedge d x^3
                \\
              & =
                \left(
                  \frac{\partial f_1}{\partial x^1}\, d x^1
                  + \frac{\partial f_1}{\partial x^2}\, d x^2
                  + \frac{\partial f_1}{\partial x^3}\, d x^3
                \right)
                \wedge d x^1 \\
              & \quad
                +
                \left(
                  \frac{\partial f_2}{\partial x^1}\, d x^1
                  + \frac{\partial f_2}{\partial x^2}\, d x^2
                  + \frac{\partial f_2}{\partial x^3}\, d x^3
                \right)
                \wedge d x^2 \\
              & \quad
                +
                \left(
                  \frac{\partial f_3}{\partial x^1}\, d x^1
                  + \frac{\partial f_3}{\partial x^2}\, d x^2
                  + \frac{\partial f_3}{\partial x^3}\, d x^3
                \right)
                \wedge d x^3
                \\
              & =
                \left(
                  \frac{\partial f_3}{\partial x^2}
                  - \frac{\partial f_2}{\partial x^3}
                \right)\,
                d x^2 \wedge d x^3
                +
                \left(
                  \frac{\partial f_1}{\partial x^3}
                  - \frac{\partial f_3}{\partial x^1}
                \right)\,
                d x^3 \wedge d x^1
                +
                \left(
                  \frac{\partial f_2}{\partial x^1}
                  - \frac{\partial f_1}{\partial x^2}
                \right)\,
                d x^1 \wedge d x^2.
            \end{split}
          \end{equation}
        \item
          \textbf{Exterior derivative of $1$-forms.}
          Consider a $2$-form $\omega \in \Omega^2(\R^3)$ such that
          \begin{equation}
            \omega
            = f_1\, d x^2 \wedge d x^3
            + f_2\, d x^3 \wedge d x^1
            + f_3\, d x^1 \wedge d x^2,
          \end{equation}
          for some $f_1, f_2, f_3 \in \mathcal{F}(\R^3)$.
          Then
          \begin{equation}
            \begin{split}
              d_2 \omega
              & = d f_1 \wedge d x^2 \wedge d x^3
                + d f_2 \wedge d x^3 \wedge d x^1
                + d f_3 \wedge d x^1 \wedge d x^2
                \\
              & =
                \left(
                  \frac{\partial f_1}{\partial x^1}\, d x^1
                  + \frac{\partial f_1}{\partial x^2}\, d x^2
                  + \frac{\partial f_1}{\partial x^3}\, d x^3
                \right)
                \wedge d x^2 \wedge d x^3 \\
              & \quad
                +
                \left(
                  \frac{\partial f_2}{\partial x^1}\, d x^1
                  + \frac{\partial f_2}{\partial x^2}\, d x^2
                  + \frac{\partial f_2}{\partial x^3}\, d x^3
                \right)
                \wedge d x^3 \wedge d x^1 \\
              & \quad
                +
                \left(
                  \frac{\partial f_3}{\partial x^1}\, d x^1
                  + \frac{\partial f_3}{\partial x^2}\, d x^2
                  + \frac{\partial f_3}{\partial x^3}\, d x^3
                \right)
                \wedge d x^1 \wedge d x^2 \\
              & =
                \left(
                  \frac{\partial f_1}{\partial x^1}
                  + \frac{\partial f_2}{\partial x^2}
                  + \frac{\partial f_3}{\partial x^3}
                \right)\,
                d x^1 \wedge d x^2 \wedge d x^3.
            \end{split}
          \end{equation}
      \end{enumerate}
  \end{enumerate}
\end{example}
