\begin{proof}
  Consider the simple tensors
  $c_1 := a_1 \otimes b_1,\ c_2 := a_2 \otimes b_2 \in A \otimes B$.
  Then
  \begin{equation}
    \begin{split}
      D(c_1 \cdot c_2)
      & = D((a_1 \otimes b_1) \cdot (a_2 \otimes b_2)) \\
      & = D((a_1 \cdot a_2) \otimes (b_1 \cdot b_2)) \\
      & = D_A(a_1 \cdot a_2) \otimes (b_1 \cdot b_2)
        + (a_1 \cdot a_2) \otimes D_B(b_1 \cdot b_2) \\
      & = (D_A a_1 \cdot a_2 + a_1 \cdot D_A a_2) \otimes (b_1 \cdot b_2)
        + (a_1 \cdot a_2) \otimes (D_B b_1 \cdot b_2 + b_1 \cdot D_B b_2) \\
      & = (D_A a_1 \otimes b_1 + a_1 \otimes D_B b_1) \cdot (a_2 \otimes b_2)
        + (a_1 \otimes b_1) \cdot (D_A a_2 \otimes b_2 + a_2 \otimes D_B b_2) \\
      & = D(a_1 \otimes b_1) \cdot (a_2 \otimes b_2)
        + (a_1 \otimes b_1) \cdot D(a_2 \otimes b_2) \\
      & = D c_1 \cdot c_2 + c_1 \cdot D c_2.
    \end{split}
  \end{equation}
  By linearity, the Leibniz rule is satisfied for all tensors.
\end{proof}
